Phi_Examples/Rational_Arith.thy
@@ -3,69 +3,105 @@ theory Rational_Arith
           Phi_Semantics.PhiSem_Int_ArbiPrec
 begin
 
-abbreviation \<open>\<r>\<a>\<t>\<i>\<o>\<n>\<a>\<l> \<equiv> \<s>\<t>\<r>\<u>\<c>\<t>{k: \<a>\<i>\<n>\<t>, v: \<a>\<i>\<n>\<t>}\<close>
+abbreviation \<open>\<r>\<a>\<t>\<i>\<o>\<n>\<a>\<l> \<equiv> \<s>\<t>\<r>\<u>\<c>\<t>{num: \<a>\<i>\<n>\<t>, den: \<a>\<i>\<n>\<t>}\<close>
 
-declare [[\<phi>trace_reasoning = 1]]
  
-\<phi>type_def \<phi>Rational :: \<open>(VAL, rat) \<phi>\<close> ("\<rat>")
-  where \<open>x \<Ztypecolon> \<phi>Rational \<equiv> (n,d) \<Ztypecolon> \<lbrace> num: \<int>, den: \<int> \<rbrace> \<s>\<u>\<b>\<j> n d. of_int n / of_int d = x \<and> d \<noteq> 0\<close>
-  deriving Basic
-       and \<open>Object_Equiv \<rat> (=)\<close>
-       and \<open>Abstract_Domain\<^sub>L \<rat> (\<lambda>_. True)\<close>
-       and \<open>Abstract_Domain \<rat> (\<lambda>_. True)\<close>
-       and Semantic_Type
-       and Inhabited
+  \<phi>type_def \<phi>Rational :: \<open>(VAL, rat) \<phi>\<close> ("\<rat>")
+    where \<open>x \<Ztypecolon> \<phi>Rational \<equiv> (n,d) \<Ztypecolon> \<lbrace> num: \<int>, den: \<int> \<rbrace>
+                       \<s>\<u>\<b>\<j> n d. of_int n / of_int d = x \<and> d \<noteq> 0\<close>
+    deriving Basic
+         and \<open>Object_Equiv \<rat> (=)\<close>
+         and \<open>Abstract_Domain\<^sub>L \<rat> (\<lambda>_. True)\<close>
+         and \<open>Abstract_Domain \<rat> (\<lambda>_. True)\<close>
+         and Semantic_Type
+         and Inhabited
 
 
-term \<open>\<v>\<a>\<l> q1 \<Ztypecolon> \<rat>\<close>
-
-proc rat_add:
-  input \<open>\<v>\<a>\<l> q1 \<Ztypecolon> \<rat> \<heavy_comma> q2 \<Ztypecolon> \<v>\<a>\<l> \<rat>\<close>
-  output \<open>q1 + q2 \<Ztypecolon> \<v>\<a>\<l> \<rat>\<close>
-\<medium_left_bracket>  
-  val q1 = (q1 \<t>\<r>\<a>\<n>\<s>\<f>\<o>\<r>\<m>\<s>_\<t>\<o> \<o>\<p>\<e>\<n>) \<semicolon>
-  val q2 = (q2 \<t>\<r>\<a>\<n>\<s>\<f>\<o>\<r>\<m>\<s>_\<t>\<o> \<o>\<p>\<e>\<n>) \<semicolon>
-  \<lbrace> num: q1.num * q2.den + q2.num * q1.den,
-    den: q1.den * q2.den \<rbrace>
-  \<m>\<a>\<k>\<e>\<s> \<open>\<rat>\<close>
-\<medium_right_bracket> .
+  proc rat_add:
+    input \<open>\<v>\<a>\<l> q1 \<Ztypecolon> \<rat> \<heavy_comma> \<v>\<a>\<l> q2 \<Ztypecolon> \<rat>\<close>
+    output \<open>\<v>\<a>\<l> q1 + q2 \<Ztypecolon> \<rat>\<close>
+  \<medium_left_bracket>  
+    val q1 = (q1 \<t>\<r>\<a>\<n>\<s>\<f>\<o>\<r>\<m>\<s>_\<t>\<o> \<o>\<p>\<e>\<n>) \<semicolon>
+    val q2 = (q2 \<t>\<r>\<a>\<n>\<s>\<f>\<o>\<r>\<m>\<s>_\<t>\<o> \<o>\<p>\<e>\<n>) \<semicolon>
+    \<lbrace> num: q1.num * q2.den + q2.num * q1.den,
+      den: q1.den * q2.den \<rbrace>
+    \<m>\<a>\<k>\<e>\<s> \<open>\<rat>\<close>
+  \<medium_right_bracket> .
 
 
-proc rat_sub:
-  input \<open>q1 \<Ztypecolon> \<v>\<a>\<l> \<rat> \<heavy_comma> q2 \<Ztypecolon> \<v>\<a>\<l> \<rat>\<close>
-  output \<open>q1 - q2 \<Ztypecolon> \<v>\<a>\<l> \<rat>\<close>
-\<medium_left_bracket>  
-  val q1 = (q1 \<t>\<r>\<a>\<n>\<s>\<f>\<o>\<r>\<m>\<s>_\<t>\<o> \<o>\<p>\<e>\<n>) \<semicolon>
-  val q2 = (q2 \<t>\<r>\<a>\<n>\<s>\<f>\<o>\<r>\<m>\<s>_\<t>\<o> \<o>\<p>\<e>\<n>) \<semicolon>
-  \<lbrace> num: q1.num * q2.den - q2.num * q1.den,
-    den: q1.den * q2.den \<rbrace>
-  \<m>\<a>\<k>\<e>\<s> \<open>\<rat>\<close>
-\<medium_right_bracket> .
+  proc rat_sub:
+    input \<open>q1 \<Ztypecolon> \<v>\<a>\<l> \<rat> \<heavy_comma> q2 \<Ztypecolon> \<v>\<a>\<l> \<rat>\<close>
+    output \<open>q1 - q2 \<Ztypecolon> \<v>\<a>\<l> \<rat>\<close>
+  \<medium_left_bracket>
+    val q1 = (q1 \<t>\<r>\<a>\<n>\<s>\<f>\<o>\<r>\<m>\<s>_\<t>\<o> \<o>\<p>\<e>\<n>) \<semicolon>
+    val q2 = (q2 \<t>\<r>\<a>\<n>\<s>\<f>\<o>\<r>\<m>\<s>_\<t>\<o> \<o>\<p>\<e>\<n>) \<semicolon>
+    \<lbrace> num: q1.num * q2.den - q2.num * q1.den,
+      den: q1.den * q2.den \<rbrace>
+    \<m>\<a>\<k>\<e>\<s> \<open>\<rat>\<close>
+  \<medium_right_bracket> .
+  
+  
+  proc rat_mul:
+    input \<open>q1 \<Ztypecolon> \<v>\<a>\<l> \<rat> \<heavy_comma> q2 \<Ztypecolon> \<v>\<a>\<l> \<rat>\<close>
+    output \<open>q1 * q2 \<Ztypecolon> \<v>\<a>\<l> \<rat>\<close>
+  \<medium_left_bracket>  
+    val q1 = (q1 \<t>\<r>\<a>\<n>\<s>\<f>\<o>\<r>\<m>\<s>_\<t>\<o> \<o>\<p>\<e>\<n>) \<semicolon>
+    val q2 = (q2 \<t>\<r>\<a>\<n>\<s>\<f>\<o>\<r>\<m>\<s>_\<t>\<o> \<o>\<p>\<e>\<n>) \<semicolon>
+    \<lbrace> num: q1.num * q2.num,
+      den: q1.den * q2.den \<rbrace>
+    \<m>\<a>\<k>\<e>\<s> \<open>\<rat>\<close>
+  \<medium_right_bracket> .
+  
+  
+  proc rat_div:
+    input \<open>\<v>\<a>\<l> q1 \<Ztypecolon> \<rat> \<heavy_comma> \<v>\<a>\<l> q2 \<Ztypecolon> \<rat>\<close>
+    premises \<open>q2 \<noteq> 0\<close>
+    output \<open>\<v>\<a>\<l> q1 / q2 \<Ztypecolon> \<rat>\<close>
+  \<medium_left_bracket>  
+    val q1 \<leftarrow> (q1 \<t>\<r>\<a>\<n>\<s>\<f>\<o>\<r>\<m>\<s>_\<t>\<o> \<o>\<p>\<e>\<n>) \<semicolon>
+    val q2 \<leftarrow> (q2 \<t>\<r>\<a>\<n>\<s>\<f>\<o>\<r>\<m>\<s>_\<t>\<o> \<o>\<p>\<e>\<n>) \<semicolon>
+    \<lbrace> num: q1.num * q2.den,
+      den: q1.den * q2.num \<rbrace>
+    \<m>\<a>\<k>\<e>\<s> \<open>\<rat>\<close>
+  \<medium_right_bracket> .
 
 
-proc rat_mul:
-  input \<open>q1 \<Ztypecolon> \<v>\<a>\<l> \<rat> \<heavy_comma> q2 \<Ztypecolon> \<v>\<a>\<l> \<rat>\<close>
-  output \<open>q1 * q2 \<Ztypecolon> \<v>\<a>\<l> \<rat>\<close>
-\<medium_left_bracket>  
-  val q1 = (q1 \<t>\<r>\<a>\<n>\<s>\<f>\<o>\<r>\<m>\<s>_\<t>\<o> \<o>\<p>\<e>\<n>) \<semicolon>
-  val q2 = (q2 \<t>\<r>\<a>\<n>\<s>\<f>\<o>\<r>\<m>\<s>_\<t>\<o> \<o>\<p>\<e>\<n>) \<semicolon>
-  \<lbrace> num: q1.num * q2.num,
-    den: q1.den * q2.den \<rbrace>
-  \<m>\<a>\<k>\<e>\<s> \<open>\<rat>\<close>
-\<medium_right_bracket> .
-
-
-proc rat_div:
-  input \<open>q1 \<Ztypecolon> \<v>\<a>\<l> \<rat> \<heavy_comma> q2 \<Ztypecolon> \<v>\<a>\<l> \<rat>\<close>
-  premises \<open>q2 \<noteq> 0\<close>
-  output \<open>q1 / q2 \<Ztypecolon> \<v>\<a>\<l> \<rat>\<close>
-\<medium_left_bracket>  
+proc rat_lt [\<phi>overload <]:
+  input \<open>\<v>\<a>\<l> q1 \<Ztypecolon> \<rat>\<heavy_comma> \<v>\<a>\<l> q2 \<Ztypecolon> \<rat>\<close>
+  output \<open>q1 < q2 \<Ztypecolon> \<v>\<a>\<l> \<bool>\<close>
+\<medium_left_bracket>
   val q1 \<leftarrow> (q1 \<t>\<r>\<a>\<n>\<s>\<f>\<o>\<r>\<m>\<s>_\<t>\<o> \<o>\<p>\<e>\<n>) \<semicolon>
   val q2 \<leftarrow> (q2 \<t>\<r>\<a>\<n>\<s>\<f>\<o>\<r>\<m>\<s>_\<t>\<o> \<o>\<p>\<e>\<n>) \<semicolon>
-  \<lbrace> num: q1.num * q2.den,
-    den: q1.den * q2.num \<rbrace>
-  \<m>\<a>\<k>\<e>\<s> \<open>\<rat>\<close>
+  val a \<leftarrow> q1.num * q2.den \<semicolon>
+  val b \<leftarrow> q1.den * q2.num \<semicolon>
+  sel (q1.den > 0 \<oplus> q2.den > 0, a > b, a < b)
 \<medium_right_bracket> .
+
+proc rat_le [\<phi>overload \<le>]:
+  input \<open>\<v>\<a>\<l> q1 \<Ztypecolon> \<rat>\<heavy_comma> \<v>\<a>\<l> q2 \<Ztypecolon> \<rat>\<close>
+  output \<open>q1 \<le> q2 \<Ztypecolon> \<v>\<a>\<l> \<bool>\<close>
+\<medium_left_bracket>
+  val q1 \<leftarrow> (q1 \<t>\<r>\<a>\<n>\<s>\<f>\<o>\<r>\<m>\<s>_\<t>\<o> \<o>\<p>\<e>\<n>) \<semicolon>
+  val q2 \<leftarrow> (q2 \<t>\<r>\<a>\<n>\<s>\<f>\<o>\<r>\<m>\<s>_\<t>\<o> \<o>\<p>\<e>\<n>) \<semicolon>
+  val a \<leftarrow> q1.num * q2.den \<semicolon>
+  val b \<leftarrow> q1.den * q2.num \<semicolon>
+  sel (q1.den > 0 \<oplus> q2.den > 0, a \<ge> b, a \<le> b)
+\<medium_right_bracket>  .
+
+proc rat_gt [\<phi>overload >]:
+  input \<open>\<v>\<a>\<l> q1 \<Ztypecolon> \<rat>\<heavy_comma> \<v>\<a>\<l> q2 \<Ztypecolon> \<rat>\<close>
+  output \<open>q1 > q2 \<Ztypecolon> \<v>\<a>\<l> \<bool>\<close>
+\<medium_left_bracket>
+  q2 < q1
+\<medium_right_bracket> .
+
+proc rat_ge [\<phi>overload >]:
+  input \<open>\<v>\<a>\<l> q1 \<Ztypecolon> \<rat>\<heavy_comma> \<v>\<a>\<l> q2 \<Ztypecolon> \<rat>\<close>
+  output \<open>q1 \<ge> q2 \<Ztypecolon> \<v>\<a>\<l> \<bool>\<close>
+\<medium_left_bracket>
+  q2 \<le> q1
+\<medium_right_bracket> .
+
 
 text \<open>The Conclusions of above Certification is the following Specification Theorems\<close>
 
